src/concurrency/DNS.ShellScheduler.fst
@@ -70,7 +70,14 @@ val dispatch_shell_event :
   ST unit
     (requires (fun h0 ->
       shell_event_live h0 event))
-    (ensures (fun _h0 _ _h1 -> True))
+    (ensures (fun h0 _ h1 ->
+      match event with
+      | AuthenticatedStreamData ctx_ptr _fragment ->
+          (let ctx = FStar.Seq.index (LowStar.Buffer.as_seq h0 ctx_ptr) 0 in
+           modifies (loc_union (loc_buffer ctx_ptr) (loc_buffer ctx.sc_buf)) h0 h1) /\
+          live h1 ctx_ptr
+      | ProcessingReady _conn _response_buffer _response_capacity _stream_id -> True
+      | ResponseSendFinished _conn _descriptor _outcome -> True))
 
 let dispatch_shell_event auth stream_borrow completion_borrow event =
   match event with
@@ -86,3 +93,107 @@ let dispatch_shell_event auth stream_borrow completion_borrow event =
       WORKER.worker_loop conn response_buffer response_capacity stream_id
   | ResponseSendFinished conn descriptor outcome ->
       COMPLETE.complete_response_send completion_borrow conn descriptor outcome
+
+val dispatch_authenticated_stream_data_event :
+  ctx_ptr:buffer stream_context ->
+  stream_id:FStar.UInt64.t ->
+  data:buffer FStar.UInt8.t ->
+  len:FStar.UInt32.t ->
+  ST stream_phase
+    (requires (fun h0 ->
+      INGRESS.authenticated_stream_fragment_live h0 ctx_ptr {
+        INGRESS.msif_stream_id = stream_id;
+        INGRESS.msif_data = data;
+        INGRESS.msif_len = len;
+        INGRESS.msif_fin = false;
+      }))
+    (ensures (fun h0 _ h1 ->
+      (let ctx = FStar.Seq.index (LowStar.Buffer.as_seq h0 ctx_ptr) 0 in
+       modifies (loc_union (loc_buffer ctx_ptr) (loc_buffer ctx.sc_buf)) h0 h1) /\
+      live h1 ctx_ptr))
+
+let dispatch_authenticated_stream_data_event ctx_ptr stream_id data len =
+  let fragment = {
+    INGRESS.msif_stream_id = stream_id;
+    INGRESS.msif_data = data;
+    INGRESS.msif_len = len;
+    INGRESS.msif_fin = false;
+  } in
+  INGRESS.handle_authenticated_stream_fragment () () ctx_ptr fragment
+
+val dispatch_minimal_worker_error_response_event :
+  conn:buffer connection_context ->
+  response_buffer:buffer FStar.UInt8.t ->
+  response_capacity:FStar.UInt32.t ->
+  stream_id:FStar.UInt64.t ->
+  ST FStar.UInt32.t
+    (requires (fun h0 ->
+      live h0 conn /\
+      LowStar.Buffer.length conn >= 1 /\
+      live h0 response_buffer /\
+      FStar.UInt32.v response_capacity <= LowStar.Buffer.length response_buffer /\
+      loc_disjoint (loc_buffer conn) (loc_buffer response_buffer) /\
+      (let c = FStar.Seq.index (LowStar.Buffer.as_seq h0 conn) 0 in
+       FStar.UInt32.v c.cc_num <= FStar.UInt32.v c.cc_capacity /\
+       (if FStar.UInt32.v c.cc_num > 0 then
+          active_streams_live h0 c.cc_active c.cc_capacity /\
+          loc_disjoint (loc_buffer conn) (loc_buffer c.cc_active)
+        else True))))
+    (ensures (fun h0 _ h1 ->
+      modifies (loc_buffer response_buffer) h0 h1 /\
+      live h1 response_buffer))
+
+let dispatch_minimal_worker_error_response_event conn response_buffer response_capacity stream_id =
+  match find_stream conn stream_id with
+  | Some ctx_ptr ->
+      let stream = LowStar.Buffer.index ctx_ptr 0ul in
+      begin match stream.sc_phase with
+      | Processing request_len ->
+          let request_len32 = FStar.UInt32.uint_to_t (FStar.UInt16.v request_len) in
+          WORKER.prepare_worker_minimal_error_response_send
+            ctx_ptr
+            response_buffer
+            response_capacity
+            request_len32
+      | _ -> 0ul
+      end
+  | None -> 0ul
+
+val dispatch_response_send_finished_for_stream_event :
+  conn:buffer connection_context ->
+  response_buffer:buffer FStar.UInt8.t ->
+  response_len:FStar.UInt32.t ->
+  stream_id:FStar.UInt64.t ->
+  outcome_code:FStar.UInt8.t ->
+  ST FStar.UInt8.t
+    (requires (fun h0 ->
+      live h0 conn /\
+      LowStar.Buffer.length conn >= 1 /\
+      live h0 response_buffer /\
+      FStar.UInt32.v response_len <= LowStar.Buffer.length response_buffer /\
+      (let c = FStar.Seq.index (LowStar.Buffer.as_seq h0 conn) 0 in
+       FStar.UInt32.v c.cc_num <= FStar.UInt32.v c.cc_capacity /\
+       (FStar.UInt32.v c.cc_num > 0 ==>
+        active_streams_live h0 c.cc_active c.cc_capacity /\
+        loc_disjoint (loc_buffer conn) (loc_buffer c.cc_active)))))
+    (ensures (fun _h0 _ _h1 -> True))
+
+let dispatch_response_send_finished_for_stream_event
+  conn
+  response_buffer
+  response_len
+  stream_id
+  outcome_code =
+  let descriptor = {
+    EGRESS.mssd_stream_id = stream_id;
+    EGRESS.mssd_data = response_buffer;
+    EGRESS.mssd_len = response_len;
+    EGRESS.mssd_fin = true;
+  } in
+  let outcome =
+    if FStar.UInt8.v outcome_code = 0 then
+      COMPLETE.SendCompleted
+    else
+      COMPLETE.SendDropped in
+  COMPLETE.complete_response_send () conn descriptor outcome;
+  1uy
